moving buffer bigops to .fsti so that all types of buffers can use them, and reducing dependent tuple also for all_live

examples/low-mitls-experiments/ImmutableBuffer.fst
@@ -106,6 +106,20 @@ let test_ub () :HST.St unit =
   assert (Seq.index (UB.as_seq h0 b) 1 == Seq.index (Seq.slice (UB.as_seq h0 b) 0 2) 1);
   assert (j == 2)
 
+
+(***** Tests for bigops in the buffer library *****)
+#push-options "--max_fuel 0 --max_ifuel 0"
+let test_bigops (b1:UB.ubuffer int) (b2:IB.ibuffer int) (b3:B.buffer int) (h h0 h1:HS.mem) : unit =
+  let open LowStar.Buffer in
+  let l1, l2, l3 = loc_buffer b1, loc_buffer b2, loc_buffer b3 in
+  assume (live h b1 /\ live h b2 /\ live h b3);
+  assume (loc_disjoint l1 l2 /\ loc_disjoint l2 l3 /\ loc_disjoint l3 l1);
+  assume (modifies (loc_union l1 (loc_union l2 l3)) h0 h1);
+  assert (all_disjoint [l1; l2; l3]);
+  assert (all_live h [buf b1; buf b2; buf b3]);
+  assert (modifies (loc_union_l [l1; l2; l3]) h0 h1)
+#pop-options
+
 // (*
 //  * An example of a two elements buffer
 //  * The first element increases monotonically and the second element remains same
